Refactoring of Constprop and Constpropproof into a machine-dependent part and a machine-independent part.
git-svn-id: https://yquem.inria.fr/compcert/svn/compcert/trunk@1126 fca1b0fc-160b-0410-b1d3-a4f43f01ea2e

arm/ConstpropOp.v
@@ -10,22 +10,16 @@
 (*                                                                     *)
 (* *********************************************************************)
 
-(** Constant propagation over RTL.  This is the first of the two
-  optimizations performed at RTL level.  It proceeds by a standard
-  dataflow analysis and the corresponding code transformation. *)
+(** Static analysis and strength reduction for operators 
+  and conditions.  This is the machine-dependent part of [Constprop]. *)
 
 Require Import Coqlib.
-Require Import Maps.
 Require Import AST.
 Require Import Integers.
 Require Import Floats.
 Require Import Values.
-Require Import Globalenvs.
 Require Import Op.
 Require Import Registers.
-Require Import RTL.
-Require Import Lattice.
-Require Import Kildall.
 
 (** * Static analysis *)
 
@@ -41,77 +35,6 @@ Inductive approx : Type :=
   | S: ident -> int -> approx.
                          (** The value is the address of the given global
                              symbol plus the given integer offset. *)
-
-(** We equip this set of approximations with a semi-lattice structure.
-  The ordering is inclusion between the sets of values denoted by
-  the approximations. *)
-
-Module Approx <: SEMILATTICE_WITH_TOP.
-  Definition t := approx.
-  Definition eq (x y: t) := (x = y).
-  Definition eq_refl: forall x, eq x x := (@refl_equal t).
-  Definition eq_sym: forall x y, eq x y -> eq y x := (@sym_equal t).
-  Definition eq_trans: forall x y z, eq x y -> eq y z -> eq x z := (@trans_equal t).
-  Lemma eq_dec: forall (x y: t), {x=y} + {x<>y}.
-  Proof.
-    decide equality.
-    apply Int.eq_dec.
-    apply Float.eq_dec.
-    apply Int.eq_dec.
-    apply ident_eq.
-  Qed.
-  Definition beq (x y: t) := if eq_dec x y then true else false.
-  Lemma beq_correct: forall x y, beq x y = true -> x = y.
-  Proof.
-    unfold beq; intros.  destruct (eq_dec x y). auto. congruence.
-  Qed.
-  Definition ge (x y: t) : Prop :=
-    x = Unknown \/ y = Novalue \/ x = y.
-  Lemma ge_refl: forall x y, eq x y -> ge x y.
-  Proof.
-    unfold eq, ge; tauto.
-  Qed.
-  Lemma ge_trans: forall x y z, ge x y -> ge y z -> ge x z.
-  Proof.
-    unfold ge; intuition congruence.
-  Qed.
-  Lemma ge_compat: forall x x' y y', eq x x' -> eq y y' -> ge x y -> ge x' y'.
-  Proof.
-    unfold eq, ge; intros; congruence.
-  Qed.
-  Definition bot := Novalue.
-  Definition top := Unknown.
-  Lemma ge_bot: forall x, ge x bot.
-  Proof.
-    unfold ge, bot; tauto.
-  Qed.
-  Lemma ge_top: forall x, ge top x.
-  Proof.
-    unfold ge, bot; tauto.
-  Qed.
-  Definition lub (x y: t) : t :=
-    if eq_dec x y then x else
-    match x, y with
-    | Novalue, _ => y
-    | _, Novalue => x
-    | _, _ => Unknown
-    end.
-  Lemma lub_commut: forall x y, eq (lub x y) (lub y x).
-  Proof.
-    unfold lub, eq; intros.
-    case (eq_dec x y); case (eq_dec y x); intros; try congruence.
-    destruct x; destruct y; auto.
-  Qed.
-  Lemma ge_lub_left: forall x y, ge (lub x y) x.
-  Proof.
-    unfold lub; intros.
-    case (eq_dec x y); intro.
-    apply ge_refl. apply eq_refl.
-    destruct x; destruct y; unfold ge; tauto.
-  Qed.
-End Approx.
-
-Module D := LPMap Approx.
 
 (** We now define the abstract interpretations of conditions and operators
   over this set of approximations.  For instance, the abstract interpretation
@@ -658,59 +581,7 @@ Definition eval_static_operation (op: operation) (vl: list approx) :=
       Unknown
   end.
 
-
-(** The transfer function for the dataflow analysis is straightforward:
-  for [Iop] instructions, we set the approximation of the destination
-  register to the result of executing abstractly the operation;
-  for [Iload] and [Icall], we set the approximation of the destination
-  to [Unknown]. *)
-
-Definition approx_regs (rl: list reg) (approx: D.t) :=
-  List.map (fun r => D.get r approx) rl.
-
-Definition transfer (f: function) (pc: node) (before: D.t) :=
-  match f.(fn_code)!pc with
-  | None => before
-  | Some i =>
-      match i with
-      | Inop s =>
-          before
-      | Iop op args res s =>
-          let a := eval_static_operation op (approx_regs args before) in
-          D.set res a before
-      | Iload chunk addr args dst s =>
-          D.set dst Unknown before
-      | Istore chunk addr args src s =>
-          before
-      | Icall sig ros args res s =>
-          D.set res Unknown before
-      | Itailcall sig ros args =>
-          before
-      | Icond cond args ifso ifnot =>
-          before
-      | Ireturn optarg =>
-          before
-      end
-  end.
-
-(** The static analysis itself is then an instantiation of Kildall's
-  generic solver for forward dataflow inequations. [analyze f]
-  returns a mapping from program points to mappings of pseudo-registers
-  to approximations.  It can fail to reach a fixpoint in a reasonable
-  number of iterations, in which case [None] is returned. *)
-
-Module DS := Dataflow_Solver(D)(NodeSetForward).
-
-Definition analyze (f: RTL.function): PMap.t D.t :=
-  match DS.fixpoint (successors f) (transfer f) 
-                    ((f.(fn_entrypoint), D.top) :: nil) with
-  | None => PMap.init D.top
-  | Some res => res
-  end.
-
-(** * Code transformation *)
-
-(** ** Operator strength reduction *)
+(** * Operator strength reduction *)
 
 (** We now define auxiliary functions for strength reduction of
   operators and addressing modes: replacing an operator with a cheaper
@@ -719,10 +590,10 @@ Definition analyze (f: RTL.function): PMap.t D.t :=
 
 Section STRENGTH_REDUCTION.
 
-Variable approx: D.t.
+Variable app: reg -> approx.
 
 Definition intval (r: reg) : option int :=
-  match D.get r approx with I n => Some n | _ => None end.
+  match app r with I n => Some n | _ => None end.
 
 (*
 Definition cond_strength_reduction (cond: condition) (args: list reg) :=
@@ -1159,77 +1030,3 @@ Definition addr_strength_reduction (addr: addressing) (args: list reg) :=
   end.
 
 End STRENGTH_REDUCTION.
-
-(** ** Code transformation *)
-
-(** The code transformation proceeds instruction by instruction.
-    Operators whose arguments are all statically known are turned
-    into ``load integer constant'', ``load float constant'' or
-    ``load symbol address'' operations.  Operators for which some
-    but not all arguments are known are subject to strength reduction,
-    and similarly for the addressing modes of load and store instructions.
-    Other instructions are unchanged. *)
-
-Definition transf_ros (approx: D.t) (ros: reg + ident) : reg + ident :=
-  match ros with
-  | inl r =>
-      match D.get r approx with
-      | S symb ofs => if Int.eq ofs Int.zero then inr _ symb else ros
-      | _ => ros
-      end
-  | inr s => ros
-  end.
-
-Definition transf_instr (approx: D.t) (instr: instruction) :=
-  match instr with
-  | Iop op args res s =>
-      match eval_static_operation op (approx_regs args approx) with
-      | I n =>
-          Iop (Ointconst n) nil res s
-      | F n =>
-          Iop (Ofloatconst n) nil res s
-      | S symb ofs =>
-          Iop (Oaddrsymbol symb ofs) nil res s
-      | _ =>
-          let (op', args') := op_strength_reduction approx op args in
-          Iop op' args' res s
-      end
-  | Iload chunk addr args dst s =>
-      let (addr', args') := addr_strength_reduction approx addr args in
-      Iload chunk addr' args' dst s      
-  | Istore chunk addr args src s =>
-      let (addr', args') := addr_strength_reduction approx addr args in
-      Istore chunk addr' args' src s      
-  | Icall sig ros args res s =>
-      Icall sig (transf_ros approx ros) args res s
-  | Itailcall sig ros args =>
-      Itailcall sig (transf_ros approx ros) args
-  | Icond cond args s1 s2 =>
-      match eval_static_condition cond (approx_regs args approx) with
-      | Some b =>
-          if b then Inop s1 else Inop s2
-      | None =>
-          let (cond', args') := cond_strength_reduction approx cond args in
-          Icond cond' args' s1 s2
-      end
-  | _ =>
-      instr
-  end.
-
-Definition transf_code (approxs: PMap.t D.t) (instrs: code) : code :=
-  PTree.map (fun pc instr => transf_instr approxs!!pc instr) instrs.
-
-Definition transf_function (f: function) : function :=
-  let approxs := analyze f in
-  mkfunction
-    f.(fn_sig)
-    f.(fn_params)
-    f.(fn_stacksize)
-    (transf_code approxs f.(fn_code))
-    f.(fn_entrypoint).
-
-Definition transf_fundef (fd: fundef) : fundef :=
-  AST.transf_fundef transf_function fd.
-
-Definition transf_program (p: program) : program :=
-  transform_program transf_fundef p.
