powerpc/ConstpropOpproof.v
@@ -13,20 +13,16 @@
 (** Correctness proof for constant propagation. *)
 
 Require Import Coqlib.
-Require Import Maps.
 Require Import AST.
 Require Import Integers.
 Require Import Floats.
 Require Import Values.
-Require Import Events.
 Require Import Mem.
 Require Import Globalenvs.
-Require Import Smallstep.
 Require Import Op.
 Require Import Registers.
 Require Import RTL.
-Require Import Lattice.
-Require Import Kildall.
+Require Import ConstpropOp.
 Require Import Constprop.
 
 (** * Correctness of the static analysis *)
@@ -51,16 +47,6 @@ Definition val_match_approx (a: approx) (v: val) : Prop :=
   | _ => False
   end.
 
-Definition regs_match_approx (a: D.t) (rs: regset) : Prop :=
-  forall r, val_match_approx (D.get r a) rs#r.
-
-Lemma regs_match_approx_top:
-  forall rs, regs_match_approx D.top rs.
-Proof.
-  intros. red; intros. simpl. rewrite PTree.gempty. 
-  unfold Approx.top, val_match_approx. auto.
-Qed.
-
 Lemma val_match_approx_increasing:
   forall a1 a2 v,
   Approx.ge a1 a2 -> val_match_approx a2 v -> val_match_approx a1 v.
@@ -72,26 +58,6 @@ Proof.
   subst a2. auto.
 Qed.
 
-Lemma regs_match_approx_increasing:
-  forall a1 a2 rs,
-  D.ge a1 a2 -> regs_match_approx a2 rs -> regs_match_approx a1 rs.
-Proof.
-  unfold D.ge, regs_match_approx. intros.
-  apply val_match_approx_increasing with (D.get r a2); auto.
-Qed.
-
-Lemma regs_match_approx_update:
-  forall ra rs a v r,
-  val_match_approx a v ->
-  regs_match_approx ra rs ->
-  regs_match_approx (D.set r a ra) (rs#r <- v).
-Proof.
-  intros; red; intros. rewrite Regmap.gsspec. 
-  case (peq r0 r); intro.
-  subst r0. rewrite D.gss. auto.
-  rewrite D.gso; auto. 
-Qed.
-
 Inductive val_list_match_approx: list approx -> list val -> Prop :=
   | vlma_nil:
       val_list_match_approx nil nil
@@ -100,16 +66,6 @@ Inductive val_list_match_approx: list approx -> list val -> Prop :=
       val_match_approx a v ->
       val_list_match_approx al vl ->
       val_list_match_approx (a :: al) (v :: vl).
-
-Lemma approx_regs_val_list:
-  forall ra rs rl,
-  regs_match_approx ra rs ->
-  val_list_match_approx (approx_regs rl ra) rs##rl.
-Proof.
-  induction rl; simpl; intros.
-  constructor.
-  constructor. apply H. auto.
-Qed.
 
 Ltac SimplVMA :=
   match goal with
@@ -214,42 +170,6 @@ Proof.
   auto.
 Qed.
 
-(** The correctness of the static analysis follows from the results
-  above and the fact that the result of the static analysis is
-  a solution of the forward dataflow inequations. *)
-
-Lemma analyze_correct_1:
-  forall f pc rs pc' i,
-  f.(fn_code)!pc = Some i ->
-  In pc' (successors_instr i) ->
-  regs_match_approx (transfer f pc (analyze f)!!pc) rs ->
-  regs_match_approx (analyze f)!!pc' rs.
-Proof.
-  intros until i. unfold analyze. 
-  caseEq (DS.fixpoint (successors f) (transfer f)
-                      ((fn_entrypoint f, D.top) :: nil)).
-  intros approxs; intros.
-  apply regs_match_approx_increasing with (transfer f pc approxs!!pc).
-  eapply DS.fixpoint_solution; eauto.
-  unfold successors_list, successors. rewrite PTree.gmap. rewrite H0. auto.
-  auto.
-  intros. rewrite PMap.gi. apply regs_match_approx_top. 
-Qed.
-
-Lemma analyze_correct_3:
-  forall f rs,
-  regs_match_approx (analyze f)!!(f.(fn_entrypoint)) rs.
-Proof.
-  intros. unfold analyze. 
-  caseEq (DS.fixpoint (successors f) (transfer f)
-                      ((fn_entrypoint f, D.top) :: nil)).
-  intros approxs; intros.
-  apply regs_match_approx_increasing with D.top.
-  eapply DS.fixpoint_entry; eauto. auto with coqlib.
-  apply regs_match_approx_top. 
-  intros. rewrite PMap.gi. apply regs_match_approx_top.
-Qed.
-
 (** * Correctness of strength reduction *)
 
 (** We now show that strength reduction over operators and addressing
@@ -260,39 +180,39 @@ Qed.
 
 Section STRENGTH_REDUCTION.
 
-Variable approx: D.t.
+Variable app: reg -> approx.
 Variable sp: val.
 Variable rs: regset.
-Hypothesis MATCH: regs_match_approx approx rs.
+Hypothesis MATCH: forall r, val_match_approx (app r) rs#r.
 
 Lemma intval_correct:
   forall r n,
-  intval approx r = Some n -> rs#r = Vint n.
+  intval app r = Some n -> rs#r = Vint n.
 Proof.
   intros until n.
-  unfold intval. caseEq (D.get r approx); intros; try discriminate.
+  unfold intval. caseEq (app r); intros; try discriminate.
   generalize (MATCH r). unfold val_match_approx. rewrite H.
   congruence. 
 Qed.
 
 Lemma cond_strength_reduction_correct:
   forall cond args,
-  let (cond', args') := cond_strength_reduction approx cond args in
+  let (cond', args') := cond_strength_reduction app cond args in
   eval_condition cond' rs##args' = eval_condition cond rs##args.
 Proof.
   intros. unfold cond_strength_reduction.
   case (cond_strength_reduction_match cond args); intros.
-  caseEq (intval approx r1); intros.
+  caseEq (intval app r1); intros.
   simpl. rewrite (intval_correct _ _ H). 
   destruct (rs#r2); auto. rewrite Int.swap_cmp. auto.
   destruct c; reflexivity.
-  caseEq (intval approx r2); intros.
+  caseEq (intval app r2); intros.
   simpl. rewrite (intval_correct _ _ H0). auto.
   auto.
-  caseEq (intval approx r1); intros.
+  caseEq (intval app r1); intros.
   simpl. rewrite (intval_correct _ _ H). 
   destruct (rs#r2); auto. rewrite Int.swap_cmpu. auto.
-  caseEq (intval approx r2); intros.
+  caseEq (intval app r2); intros.
   simpl. rewrite (intval_correct _ _ H0). auto.
   auto.
   auto.
@@ -414,26 +334,26 @@ Qed.
 
 Lemma op_strength_reduction_correct:
   forall op args v,
-  let (op', args') := op_strength_reduction approx op args in
+  let (op', args') := op_strength_reduction app op args in
   eval_operation ge sp op rs##args = Some v ->
   eval_operation ge sp op' rs##args' = Some v.
 Proof.
   intros; unfold op_strength_reduction;
   case (op_strength_reduction_match op args); intros; simpl List.map.
   (* Oadd *)
-  caseEq (intval approx r1); intros.
+  caseEq (intval app r1); intros.
   rewrite (intval_correct _ _ H). 
   replace (eval_operation ge sp Oadd (Vint i :: rs # r2 :: nil))
      with (eval_operation ge sp Oadd (rs # r2 :: Vint i :: nil)).
   apply make_addimm_correct. 
   simpl. destruct rs#r2; auto. rewrite Int.add_commut; auto.
-  caseEq (intval approx r2); intros.
+  caseEq (intval app r2); intros.
   rewrite (intval_correct _ _ H0). apply make_addimm_correct.
   assumption.
   (* Osub *)
-  caseEq (intval approx r1); intros.
+  caseEq (intval app r1); intros.
   rewrite (intval_correct _ _ H) in H0. assumption. 
-  caseEq (intval approx r2); intros.
+  caseEq (intval app r2); intros.
   rewrite (intval_correct _ _ H0). 
   replace (eval_operation ge sp Osub (rs # r1 :: Vint i :: nil))
      with (eval_operation ge sp Oadd (rs # r1 :: Vint (Int.neg i) :: nil)).
@@ -441,17 +361,17 @@ Proof.
   simpl. destruct rs#r1; auto; rewrite Int.sub_add_opp; auto. 
   assumption.
   (* Omul *)
-  caseEq (intval approx r1); intros.
+  caseEq (intval app r1); intros.
   rewrite (intval_correct _ _ H). 
   replace (eval_operation ge sp Omul (Vint i :: rs # r2 :: nil))
      with (eval_operation ge sp Omul (rs # r2 :: Vint i :: nil)).
   apply make_mulimm_correct. 
   simpl. destruct rs#r2; auto. rewrite Int.mul_commut; auto.
-  caseEq (intval approx r2); intros.
+  caseEq (intval app r2); intros.
   rewrite (intval_correct _ _ H0). apply make_mulimm_correct.
   assumption.
   (* Odiv *)
-  caseEq (intval approx r2); intros.
+  caseEq (intval app r2); intros.
   caseEq (Int.is_power2 i); intros.
   rewrite (intval_correct _ _ H) in H1.   
   simpl in *; FuncInv. destruct (Int.eq i Int.zero). congruence.
@@ -461,7 +381,7 @@ Proof.
   assumption.
   assumption.
   (* Odivu *)
-  caseEq (intval approx r2); intros.
+  caseEq (intval app r2); intros.
   caseEq (Int.is_power2 i); intros.
   rewrite (intval_correct _ _ H).
   replace (eval_operation ge sp Odivu (rs # r1 :: Vint i :: nil))
@@ -476,56 +396,56 @@ Proof.
   assumption.
   assumption.
   (* Oand *)
-  caseEq (intval approx r1); intros.
+  caseEq (intval app r1); intros.
   rewrite (intval_correct _ _ H). 
   replace (eval_operation ge sp Oand (Vint i :: rs # r2 :: nil))
      with (eval_operation ge sp Oand (rs # r2 :: Vint i :: nil)).
   apply make_andimm_correct. 
   simpl. destruct rs#r2; auto. rewrite Int.and_commut; auto.
-  caseEq (intval approx r2); intros.
+  caseEq (intval app r2); intros.
   rewrite (intval_correct _ _ H0). apply make_andimm_correct.
   assumption.
   (* Oor *)
-  caseEq (intval approx r1); intros.
+  caseEq (intval app r1); intros.
   rewrite (intval_correct _ _ H). 
   replace (eval_operation ge sp Oor (Vint i :: rs # r2 :: nil))
      with (eval_operation ge sp Oor (rs # r2 :: Vint i :: nil)).
   apply make_orimm_correct. 
   simpl. destruct rs#r2; auto. rewrite Int.or_commut; auto.
-  caseEq (intval approx r2); intros.
+  caseEq (intval app r2); intros.
   rewrite (intval_correct _ _ H0). apply make_orimm_correct.
   assumption.
   (* Oxor *)
-  caseEq (intval approx r1); intros.
+  caseEq (intval app r1); intros.
   rewrite (intval_correct _ _ H). 
   replace (eval_operation ge sp Oxor (Vint i :: rs # r2 :: nil))
      with (eval_operation ge sp Oxor (rs # r2 :: Vint i :: nil)).
   apply make_xorimm_correct. 
   simpl. destruct rs#r2; auto. rewrite Int.xor_commut; auto.
-  caseEq (intval approx r2); intros.
+  caseEq (intval app r2); intros.
   rewrite (intval_correct _ _ H0). apply make_xorimm_correct.
   assumption.
   (* Oshl *)
-  caseEq (intval approx r2); intros.
+  caseEq (intval app r2); intros.
   caseEq (Int.ltu i (Int.repr 32)); intros.
   rewrite (intval_correct _ _ H). apply make_shlimm_correct.
   assumption.
   assumption.
   (* Oshr *)
-  caseEq (intval approx r2); intros.
+  caseEq (intval app r2); intros.
   caseEq (Int.ltu i (Int.repr 32)); intros.
   rewrite (intval_correct _ _ H). apply make_shrimm_correct.
   assumption.
   assumption.
   (* Oshru *)
-  caseEq (intval approx r2); intros.
+  caseEq (intval app r2); intros.
   caseEq (Int.ltu i (Int.repr 32)); intros.
   rewrite (intval_correct _ _ H). apply make_shruimm_correct.
   assumption.
   assumption.
   (* Ocmp *)
   generalize (cond_strength_reduction_correct c rl).
-  destruct (cond_strength_reduction approx c rl).
+  destruct (cond_strength_reduction app c rl).
   simpl. intro. rewrite H. auto.
   (* default *)
   assumption.
@@ -533,15 +453,14 @@ Qed.
 
 Ltac KnownApprox :=
   match goal with
-  | MATCH: (regs_match_approx ?approx ?rs),
-    H: (D.get ?r ?approx = ?a) |- _ =>
+  | H: ?approx ?r = ?a |- _ =>
       generalize (MATCH r); rewrite H; intro; clear H; KnownApprox
   | _ => idtac
   end.
  
 Lemma addr_strength_reduction_correct:
   forall addr args,
-  let (addr', args') := addr_strength_reduction approx addr args in
+  let (addr', args') := addr_strength_reduction app addr args in
   eval_addressing ge sp addr' rs##args' = eval_addressing ge sp addr rs##args.
 Proof.
   intros. 
@@ -589,18 +508,18 @@ Proof.
   case (addr_strength_reduction_match addr args); intros.
 
   (* Aindexed2 *)
-  caseEq (D.get r1 approx); intros;
-  caseEq (D.get r2 approx); intros;
+  caseEq (app r1); intros;
+  caseEq (app r2); intros;
   try reflexivity; KnownApprox; auto.
   rewrite A0. rewrite Int.add_commut. apply A5; auto.
 
   (* Abased *)
-  caseEq (intval approx r1); intros.
+  caseEq (intval app r1); intros.
   simpl; rewrite (intval_correct _ _ H). auto.
   auto.
 
   (* Aindexed *)
-  caseEq (D.get r1 approx); intros; auto.
+  caseEq (app r1); intros; auto.
   simpl; KnownApprox. 
   elim H0. intros b [A B]. rewrite A; rewrite B. auto.
 
@@ -612,330 +531,3 @@ End STRENGTH_REDUCTION.
 
 End ANALYSIS.
 
-(** * Correctness of the code transformation *)
-
-(** We now show that the transformed code after constant propagation
-  has the same semantics as the original code. *)
-
-Section PRESERVATION.
-
-Variable prog: program.
-Let tprog := transf_program prog.
-Let ge := Genv.globalenv prog.
-Let tge := Genv.globalenv tprog.
-
-Lemma symbols_preserved:
-  forall (s: ident), Genv.find_symbol tge s = Genv.find_symbol ge s.
-Proof.
-  intros; unfold ge, tge, tprog, transf_program. 
-  apply Genv.find_symbol_transf.
-Qed.
-
-Lemma functions_translated:
-  forall (v: val) (f: fundef),
-  Genv.find_funct ge v = Some f ->
-  Genv.find_funct tge v = Some (transf_fundef f).
-Proof.  
-  intros.
-  exact (Genv.find_funct_transf transf_fundef H).
-Qed.
-
-Lemma function_ptr_translated:
-  forall (b: block) (f: fundef),
-  Genv.find_funct_ptr ge b = Some f ->
-  Genv.find_funct_ptr tge b = Some (transf_fundef f).
-Proof.  
-  intros. 
-  exact (Genv.find_funct_ptr_transf transf_fundef H).
-Qed.
-
-Lemma sig_function_translated:
-  forall f,
-  funsig (transf_fundef f) = funsig f.
-Proof.
-  intros. destruct f; reflexivity.
-Qed.
-
-Lemma transf_ros_correct:
-  forall ros rs f approx,
-  regs_match_approx ge approx rs ->
-  find_function ge ros rs = Some f ->
-  find_function tge (transf_ros approx ros) rs = Some (transf_fundef f).
-Proof.
-  intros until approx; intro MATCH.
-  destruct ros; simpl.
-  intro.
-  exploit functions_translated; eauto. intro FIND.  
-  caseEq (D.get r approx); intros; auto.
-  generalize (Int.eq_spec i0 Int.zero); case (Int.eq i0 Int.zero); intros; auto.
-  generalize (MATCH r). rewrite H0. intros [b [A B]].
-  rewrite <- symbols_preserved in A.
-  rewrite B in FIND. rewrite H1 in FIND. 
-  rewrite Genv.find_funct_find_funct_ptr in FIND.
-  simpl. rewrite A. auto.
-  rewrite symbols_preserved. destruct (Genv.find_symbol ge i).
-  intro. apply function_ptr_translated. auto.
-  congruence.
-Qed.
-
-(** The proof of semantic preservation is a simulation argument
-  based on diagrams of the following form:
-<<
-           st1 --------------- st2
-            |                   |
-           t|                   |t
-            |                   |
-            v                   v
-           st1'--------------- st2'
->>
-  The left vertical arrow represents a transition in the
-  original RTL code.  The top horizontal bar is the [match_states]
-  invariant between the initial state [st1] in the original RTL code
-  and an initial state [st2] in the transformed code.
-  This invariant expresses that all code fragments appearing in [st2]
-  are obtained by [transf_code] transformation of the corresponding
-  fragments in [st1].  Moreover, the values of registers in [st1]
-  must match their compile-time approximations at the current program
-  point.
-  These two parts of the diagram are the hypotheses.  In conclusions,
-  we want to prove the other two parts: the right vertical arrow,
-  which is a transition in the transformed RTL code, and the bottom
-  horizontal bar, which means that the [match_state] predicate holds
-  between the final states [st1'] and [st2']. *)
-
-Inductive match_stackframes: stackframe -> stackframe -> Prop :=
-   match_stackframe_intro:
-      forall res c sp pc rs f,
-      c = f.(RTL.fn_code) ->
-      (forall v, regs_match_approx ge (analyze f)!!pc (rs#res <- v)) ->
-    match_stackframes
-        (Stackframe res c sp pc rs)
-        (Stackframe res (transf_code (analyze f) c) sp pc rs).
-
-Inductive match_states: state -> state -> Prop :=
-  | match_states_intro:
-      forall s c sp pc rs m f s'
-           (CF: c = f.(RTL.fn_code))
-           (MATCH: regs_match_approx ge (analyze f)!!pc rs)
-           (STACKS: list_forall2 match_stackframes s s'),
-      match_states (State s c sp pc rs m)
-                   (State s' (transf_code (analyze f) c) sp pc rs m)
-  | match_states_call:
-      forall s f args m s',
-      list_forall2 match_stackframes s s' ->
-      match_states (Callstate s f args m)
-                   (Callstate s' (transf_fundef f) args m)
-  | match_states_return:
-      forall s s' v m,
-      list_forall2 match_stackframes s s' ->
-      match_states (Returnstate s v m)
-                   (Returnstate s' v m).
-
-Ltac TransfInstr :=
-  match goal with
-  | H1: (PTree.get ?pc ?c = Some ?instr), f: function |- _ =>
-      cut ((transf_code (analyze f) c)!pc = Some(transf_instr (analyze f)!!pc instr));
-      [ simpl
-      | unfold transf_code; rewrite PTree.gmap; 
-        unfold option_map; rewrite H1; reflexivity ]
-  end.
-
-(** The proof of simulation proceeds by case analysis on the transition
-  taken in the source code. *)
-
-Lemma transf_step_correct:
-  forall s1 t s2,
-  step ge s1 t s2 ->
-  forall s1' (MS: match_states s1 s1'),
-  exists s2', step tge s1' t s2' /\ match_states s2 s2'.
-Proof.
-  induction 1; intros; inv MS.
-
-  (* Inop *)
-  exists (State s' (transf_code (analyze f) (fn_code f)) sp pc' rs m); split.
-  TransfInstr; intro. eapply exec_Inop; eauto.
-  econstructor; eauto.
-  eapply analyze_correct_1 with (pc := pc); eauto.
-  simpl; auto.
-  unfold transfer; rewrite H. auto.
-
-  (* Iop *)
-  exists (State s' (transf_code (analyze f) (fn_code f)) sp pc' (rs#res <- v) m); split.
-  TransfInstr. caseEq (op_strength_reduction (analyze f)!!pc op args);
-  intros op' args' OSR.
-  assert (eval_operation tge sp op' rs##args' = Some v).
-    rewrite (eval_operation_preserved symbols_preserved). 
-    generalize (op_strength_reduction_correct ge (analyze f)!!pc sp rs
-                  MATCH op args v).
-    rewrite OSR; simpl. auto.
-  generalize (eval_static_operation_correct ge op sp
-               (approx_regs args (analyze f)!!pc) rs##args v
-               (approx_regs_val_list _ _ _ args MATCH) H0).
-  case (eval_static_operation op (approx_regs args (analyze f)!!pc)); intros;
-  simpl in H2;
-  eapply exec_Iop; eauto; simpl.
-  congruence.
-  congruence.
-  elim H2; intros b [A B]. rewrite symbols_preserved. 
-  rewrite A; rewrite B; auto.
-  econstructor; eauto. 
-  eapply analyze_correct_1 with (pc := pc); eauto.
-  simpl; auto.
-  unfold transfer; rewrite H. 
-  apply regs_match_approx_update; auto. 
-  eapply eval_static_operation_correct; eauto.
-  apply approx_regs_val_list; auto.
-
-  (* Iload *)
-  caseEq (addr_strength_reduction (analyze f)!!pc addr args);
-  intros addr' args' ASR.
-  assert (eval_addressing tge sp addr' rs##args' = Some a).
-    rewrite (eval_addressing_preserved symbols_preserved). 
-    generalize (addr_strength_reduction_correct ge (analyze f)!!pc sp rs
-                  MATCH addr args).
-    rewrite ASR; simpl. congruence. 
-  TransfInstr. rewrite ASR. intro.
-  exists (State s' (transf_code (analyze f) (fn_code f)) sp pc' (rs#dst <- v) m); split.
-  eapply exec_Iload; eauto.
-  econstructor; eauto. 
-  eapply analyze_correct_1; eauto. simpl; auto. 
-  unfold transfer; rewrite H. 
-  apply regs_match_approx_update; auto. simpl; auto.
-
-  (* Istore *)
-  caseEq (addr_strength_reduction (analyze f)!!pc addr args);
-  intros addr' args' ASR.
-  assert (eval_addressing tge sp addr' rs##args' = Some a).
-    rewrite (eval_addressing_preserved symbols_preserved). 
-    generalize (addr_strength_reduction_correct ge (analyze f)!!pc sp rs
-                  MATCH addr args).
-    rewrite ASR; simpl. congruence. 
-  TransfInstr. rewrite ASR. intro.
-  exists (State s' (transf_code (analyze f) (fn_code f)) sp pc' rs m'); split.
-  eapply exec_Istore; eauto.
-  econstructor; eauto. 
-  eapply analyze_correct_1; eauto. simpl; auto. 
-  unfold transfer; rewrite H. auto. 
-
-  (* Icall *)
-  exploit transf_ros_correct; eauto. intro FIND'.
-  TransfInstr; intro.
-  econstructor; split.
-  eapply exec_Icall; eauto. apply sig_function_translated; auto.
-  constructor; auto. constructor; auto.
-  econstructor; eauto. 
-  intros. eapply analyze_correct_1; eauto. simpl; auto.
-  unfold transfer; rewrite H.
-  apply regs_match_approx_update; auto. simpl. auto.
-
-  (* Itailcall *)
-  exploit transf_ros_correct; eauto. intros FIND'.
-  TransfInstr; intro.
-  econstructor; split.
-  eapply exec_Itailcall; eauto. apply sig_function_translated; auto.
-  constructor; auto. 
-
-  (* Icond, true *)
-  exists (State s' (transf_code (analyze f) (fn_code f)) sp ifso rs m); split. 
-  caseEq (cond_strength_reduction (analyze f)!!pc cond args);
-  intros cond' args' CSR.
-  assert (eval_condition cond' rs##args' = Some true).
-    generalize (cond_strength_reduction_correct
-                  ge (analyze f)!!pc rs MATCH cond args).
-    rewrite CSR.  intro. congruence.
-  TransfInstr. rewrite CSR. 
-  caseEq (eval_static_condition cond (approx_regs args (analyze f)!!pc)).
-  intros b ESC. 
-  generalize (eval_static_condition_correct ge cond _ _ _
-               (approx_regs_val_list _ _ _ args MATCH) ESC); intro.
-  replace b with true. intro; eapply exec_Inop; eauto. congruence.
-  intros. eapply exec_Icond_true; eauto.
-  econstructor; eauto.
-  eapply analyze_correct_1; eauto.
-  simpl; auto.
-  unfold transfer; rewrite H; auto.
-
-  (* Icond, false *)
-  exists (State s' (transf_code (analyze f) (fn_code f)) sp ifnot rs m); split. 
-  caseEq (cond_strength_reduction (analyze f)!!pc cond args);
-  intros cond' args' CSR.
-  assert (eval_condition cond' rs##args' = Some false).
-    generalize (cond_strength_reduction_correct
-                  ge (analyze f)!!pc rs MATCH cond args).
-    rewrite CSR.  intro. congruence.
-  TransfInstr. rewrite CSR. 
-  caseEq (eval_static_condition cond (approx_regs args (analyze f)!!pc)).
-  intros b ESC. 
-  generalize (eval_static_condition_correct ge cond _ _ _
-               (approx_regs_val_list _ _ _ args MATCH) ESC); intro.
-  replace b with false. intro; eapply exec_Inop; eauto. congruence.
-  intros. eapply exec_Icond_false; eauto.
-  econstructor; eauto.
-  eapply analyze_correct_1; eauto.
-  simpl; auto.
-  unfold transfer; rewrite H; auto.
-
-  (* Ireturn *)
-  exists (Returnstate s' (regmap_optget or Vundef rs) (free m stk)); split.
-  eapply exec_Ireturn; eauto. TransfInstr; auto.
-  constructor; auto.
-
-  (* internal function *)
-  simpl. unfold transf_function.
-  econstructor; split.
-  eapply exec_function_internal; simpl; eauto.
-  simpl. econstructor; eauto.
-  apply analyze_correct_3; auto.
-
-  (* external function *)
-  simpl. econstructor; split.
-  eapply exec_function_external; eauto.
-  constructor; auto.
-
-  (* return *)
-  inv H3. inv H1. 
-  econstructor; split.
-  eapply exec_return; eauto. 
-  econstructor; eauto. 
-Qed.
-
-Lemma transf_initial_states:
-  forall st1, initial_state prog st1 ->
-  exists st2, initial_state tprog st2 /\ match_states st1 st2.
-Proof.
-  intros. inversion H.
-  exploit function_ptr_translated; eauto. intro FIND.
-  exists (Callstate nil (transf_fundef f) nil (Genv.init_mem tprog)); split.
-  econstructor; eauto.
-  replace (prog_main tprog) with (prog_main prog).
-  rewrite symbols_preserved. eauto.
-  reflexivity.
-  rewrite <- H2. apply sig_function_translated.
-  replace (Genv.init_mem tprog) with (Genv.init_mem prog).
-  constructor. constructor. auto.
-  symmetry. unfold tprog, transf_program. apply Genv.init_mem_transf. 
-Qed.
-
-Lemma transf_final_states:
-  forall st1 st2 r, 
-  match_states st1 st2 -> final_state st1 r -> final_state st2 r.
-Proof.
-  intros. inv H0. inv H. inv H4. constructor. 
-Qed.
-
-(** The preservation of the observable behavior of the program then
-  follows, using the generic preservation theorem
-  [Smallstep.simulation_step_preservation]. *)
-
-Theorem transf_program_correct:
-  forall (beh: program_behavior), not_wrong beh ->
-  exec_program prog beh -> exec_program tprog beh.
-Proof.
-  unfold exec_program; intros.
-  eapply simulation_step_preservation; eauto.
-  eexact transf_initial_states.
-  eexact transf_final_states.
-  exact transf_step_correct. 
-Qed.
-
-End PRESERVATION.
