backend/Constprop.v
@@ -1,0 +1,235 @@
+(* *********************************************************************)
+(*                                                                     *)
+(*              The Compcert verified compiler                         *)
+(*                                                                     *)
+(*          Xavier Leroy, INRIA Paris-Rocquencourt                     *)
+(*                                                                     *)
+(*  Copyright Institut National de Recherche en Informatique et en     *)
+(*  Automatique.  All rights reserved.  This file is distributed       *)
+(*  under the terms of the INRIA Non-Commercial License Agreement.     *)
+(*                                                                     *)
+(* *********************************************************************)
+
+(** Constant propagation over RTL.  This is one of the optimizations
+  performed at RTL level.  It proceeds by a standard dataflow analysis
+  and the corresponding code rewriting. *)
+
+Require Import Coqlib.
+Require Import Maps.
+Require Import AST.
+Require Import Integers.
+Require Import Floats.
+Require Import Values.
+Require Import Globalenvs.
+Require Import Op.
+Require Import Registers.
+Require Import RTL.
+Require Import Lattice.
+Require Import Kildall.
+Require Import ConstpropOp.
+
+(** * Static analysis *)
+
+(** The type [approx] of compile-time approximations of values is
+  defined in the machine-dependent part [ConstpropOp]. *)
+
+(** We equip this type of approximations with a semi-lattice structure.
+  The ordering is inclusion between the sets of values denoted by
+  the approximations. *)
+
+Module Approx <: SEMILATTICE_WITH_TOP.
+  Definition t := approx.
+  Definition eq (x y: t) := (x = y).
+  Definition eq_refl: forall x, eq x x := (@refl_equal t).
+  Definition eq_sym: forall x y, eq x y -> eq y x := (@sym_equal t).
+  Definition eq_trans: forall x y z, eq x y -> eq y z -> eq x z := (@trans_equal t).
+  Lemma eq_dec: forall (x y: t), {x=y} + {x<>y}.
+  Proof.
+    decide equality.
+    apply Int.eq_dec.
+    apply Float.eq_dec.
+    apply Int.eq_dec.
+    apply ident_eq.
+  Qed.
+  Definition beq (x y: t) := if eq_dec x y then true else false.
+  Lemma beq_correct: forall x y, beq x y = true -> x = y.
+  Proof.
+    unfold beq; intros.  destruct (eq_dec x y). auto. congruence.
+  Qed.
+  Definition ge (x y: t) : Prop :=
+    x = Unknown \/ y = Novalue \/ x = y.
+  Lemma ge_refl: forall x y, eq x y -> ge x y.
+  Proof.
+    unfold eq, ge; tauto.
+  Qed.
+  Lemma ge_trans: forall x y z, ge x y -> ge y z -> ge x z.
+  Proof.
+    unfold ge; intuition congruence.
+  Qed.
+  Lemma ge_compat: forall x x' y y', eq x x' -> eq y y' -> ge x y -> ge x' y'.
+  Proof.
+    unfold eq, ge; intros; congruence.
+  Qed.
+  Definition bot := Novalue.
+  Definition top := Unknown.
+  Lemma ge_bot: forall x, ge x bot.
+  Proof.
+    unfold ge, bot; tauto.
+  Qed.
+  Lemma ge_top: forall x, ge top x.
+  Proof.
+    unfold ge, bot; tauto.
+  Qed.
+  Definition lub (x y: t) : t :=
+    if eq_dec x y then x else
+    match x, y with
+    | Novalue, _ => y
+    | _, Novalue => x
+    | _, _ => Unknown
+    end.
+  Lemma lub_commut: forall x y, eq (lub x y) (lub y x).
+  Proof.
+    unfold lub, eq; intros.
+    case (eq_dec x y); case (eq_dec y x); intros; try congruence.
+    destruct x; destruct y; auto.
+  Qed.
+  Lemma ge_lub_left: forall x y, ge (lub x y) x.
+  Proof.
+    unfold lub; intros.
+    case (eq_dec x y); intro.
+    apply ge_refl. apply eq_refl.
+    destruct x; destruct y; unfold ge; tauto.
+  Qed.
+End Approx.
+
+Module D := LPMap Approx.
+
+(** The transfer function for the dataflow analysis is straightforward:
+  for [Iop] instructions, we set the approximation of the destination
+  register to the result of executing abstractly the operation;
+  for [Iload] and [Icall], we set the approximation of the destination
+  to [Unknown]. *)
+
+Definition approx_reg (app: D.t) (r: reg) := 
+  D.get r app.
+
+Definition approx_regs (app: D.t) (rl: list reg):=
+  List.map (approx_reg app) rl.
+
+Definition transfer (f: function) (pc: node) (before: D.t) :=
+  match f.(fn_code)!pc with
+  | None => before
+  | Some i =>
+      match i with
+      | Inop s =>
+          before
+      | Iop op args res s =>
+          let a := eval_static_operation op (approx_regs before args) in
+          D.set res a before
+      | Iload chunk addr args dst s =>
+          D.set dst Unknown before
+      | Istore chunk addr args src s =>
+          before
+      | Icall sig ros args res s =>
+          D.set res Unknown before
+      | Itailcall sig ros args =>
+          before
+(*
+      | Ialloc arg res s =>
+          D.set res Unknown before
+*)
+      | Icond cond args ifso ifnot =>
+          before
+      | Ireturn optarg =>
+          before
+      end
+  end.
+
+(** The static analysis itself is then an instantiation of Kildall's
+  generic solver for forward dataflow inequations. [analyze f]
+  returns a mapping from program points to mappings of pseudo-registers
+  to approximations.  It can fail to reach a fixpoint in a reasonable
+  number of iterations, in which case [None] is returned. *)
+
+Module DS := Dataflow_Solver(D)(NodeSetForward).
+
+Definition analyze (f: RTL.function): PMap.t D.t :=
+  match DS.fixpoint (successors f) (transfer f) 
+                    ((f.(fn_entrypoint), D.top) :: nil) with
+  | None => PMap.init D.top
+  | Some res => res
+  end.
+
+(** * Code transformation *)
+
+(** The code transformation proceeds instruction by instruction.
+    Operators whose arguments are all statically known are turned
+    into ``load integer constant'', ``load float constant'' or
+    ``load symbol address'' operations.  Operators for which some
+    but not all arguments are known are subject to strength reduction,
+    and similarly for the addressing modes of load and store instructions.
+    Other instructions are unchanged. *)
+
+Definition transf_ros (app: D.t) (ros: reg + ident) : reg + ident :=
+  match ros with
+  | inl r =>
+      match D.get r app with
+      | S symb ofs => if Int.eq ofs Int.zero then inr _ symb else ros
+      | _ => ros
+      end
+  | inr s => ros
+  end.
+
+Definition transf_instr (app: D.t) (instr: instruction) :=
+  match instr with
+  | Iop op args res s =>
+      match eval_static_operation op (approx_regs app args) with
+      | I n =>
+          Iop (Ointconst n) nil res s
+      | F n =>
+          Iop (Ofloatconst n) nil res s
+      | S symb ofs =>
+          Iop (Oaddrsymbol symb ofs) nil res s
+      | _ =>
+          let (op', args') := op_strength_reduction (approx_reg app) op args in
+          Iop op' args' res s
+      end
+  | Iload chunk addr args dst s =>
+      let (addr', args') := addr_strength_reduction (approx_reg app) addr args in
+      Iload chunk addr' args' dst s      
+  | Istore chunk addr args src s =>
+      let (addr', args') := addr_strength_reduction (approx_reg app) addr args in
+      Istore chunk addr' args' src s      
+  | Icall sig ros args res s =>
+      Icall sig (transf_ros app ros) args res s
+  | Itailcall sig ros args =>
+      Itailcall sig (transf_ros app ros) args
+  | Icond cond args s1 s2 =>
+      match eval_static_condition cond (approx_regs app args) with
+      | Some b =>
+          if b then Inop s1 else Inop s2
+      | None =>
+          let (cond', args') := cond_strength_reduction (approx_reg app) cond args in
+          Icond cond' args' s1 s2
+      end
+  | _ =>
+      instr
+  end.
+
+Definition transf_code (approxs: PMap.t D.t) (instrs: code) : code :=
+  PTree.map (fun pc instr => transf_instr approxs!!pc instr) instrs.
+
+Definition transf_function (f: function) : function :=
+  let approxs := analyze f in
+  mkfunction
+    f.(fn_sig)
+    f.(fn_params)
+    f.(fn_stacksize)
+    (transf_code approxs f.(fn_code))
+    f.(fn_entrypoint).
+
+Definition transf_fundef (fd: fundef) : fundef :=
+  AST.transf_fundef transf_function fd.
+
+Definition transf_program (p: program) : program :=
+  transform_program transf_fundef p.
